src/program_proof/pav/should_build.v
@@ -10,4 +10,4 @@ From Perennial.program_proof.pav Require
   merkle_internal
   misc
   rpc
-  (* server *).
+  server.
